AtomicRegThm.v
@@ -1,6 +1,6 @@
 Set Implicit Arguments.
 
-Require Import AtomicReg AtomicRegIfc StoreAtomicity DataTypes.
+Require Import AtomicReg AtomicRegIfc StoreAtomicity DataTypes Transitions.
 
 Section ForAddr.
   Variable reqFn: Addr -> Cache -> Index -> Req.
@@ -8,19 +8,15 @@ Section ForAddr.
 
   Variable sa: StoreAtomicity reqFn respFn.
 
-  Theorem storeAtomicityImpAtomicRegBehavior n :
-    exists (al: AtomicTransList reqFn (Build_State (initData) (fun a t => 0))),
-      respFn n = getResp n al.
+  Theorem atomicRegSimulateCaches n :
+    exists (al: Stream (AtomicTrans reqFn) (Build_State (initData) (fun a t => 0))),
+      getCacheIo reqFn respFn n = getStreamIo (@getTransIo reqFn ) n al.
   Proof.
     exists (buildAl reqFn respFn 0).
     About getRespEq.
-    pose proof (getRespEq sa n) as e1.
-    pose proof (respEq sa n) as e2.
+    pose proof (getIoEq sa n) as e1.
+    pose proof (ioEq sa n) as e2.
     rewrite <- e1 in e2.
     assumption.
   Qed.
 End ForAddr.
-
-Print Assumptions storeAtomicityImpAtomicRegBehavior.
-
-About storeAtomicityImpAtomicRegBehavior.
